proof/Ring_ops_proof_ct.ec
@@ -1,7 +1,8 @@
 require import Ring_ops_extract_ct.
-
+require import JModel List Int AllCore.
 
 equiv expm_ct :
   M.expm ~ M.expm :
   ={M.leakages, glob M} ==> ={M.leakages}.
 proof. proc; inline *; sim. qed.
+
