proof/Ring_ops_spec.ec
@@ -39,6 +39,7 @@ clone import ZModP.ZModRing as Zp with
         op p <= P
         rename "zmod" as "zp".
 
+
         
 (** "Implements" relation *)
 abbrev ImplWord x y = W64.to_uint x = y.
