proof/Uniform_distr_extract_ct.ec
@@ -1,0 +1,145 @@
+require import AllCore IntDiv CoreMap List Distr.
+require import JModel.
+
+require import Array32 Array256.
+require import WArray256.
+
+
+
+module type Syscall_t = {
+  proc randombytes_256(_:W8.t Array256.t) : W8.t Array256.t
+}.
+
+module Syscall : Syscall_t = {
+  proc randombytes_256(a:W8.t Array256.t) : W8.t Array256.t = {
+    a <$ dmap WArray256.darray
+         (fun a => Array256.init (fun i => WArray256.get8 a i));
+    return a;
+  }
+}.
+
+module M(SC:Syscall_t) = {
+  var leakages : leakages_t
+  
+  proc bn_subc (a:W64.t Array32.t, b:W64.t Array32.t) : bool *
+                                                        W64.t Array32.t = {
+    var aux_0: bool;
+    var aux_1: int;
+    var aux: W64.t;
+    
+    var cf:bool;
+    var x1:W64.t;
+    var x2:W64.t;
+    var i:int;
+    
+    leakages <- LeakAddr([0]) :: leakages;
+    aux <- a.[0];
+    x1 <- aux;
+    leakages <- LeakAddr([0]) :: leakages;
+    aux <- b.[0];
+    x2 <- aux;
+    leakages <- LeakAddr([]) :: leakages;
+    (aux_0, aux) <- subc_64 x1 x2 false;
+    cf <- aux_0;
+    x1 <- aux;
+    leakages <- LeakAddr([]) :: leakages;
+    aux <- x1;
+    leakages <- LeakAddr([0]) :: leakages;
+    a.[0] <- aux;
+    leakages <- LeakFor(1,32) :: LeakAddr([]) :: leakages;
+    i <- 1;
+    while (i < 32) {
+      leakages <- LeakAddr([i]) :: leakages;
+      aux <- a.[i];
+      x1 <- aux;
+      leakages <- LeakAddr([i]) :: leakages;
+      aux <- b.[i];
+      x2 <- aux;
+      leakages <- LeakAddr([]) :: leakages;
+      (aux_0, aux) <- subc_64 x1 x2 cf;
+      cf <- aux_0;
+      x1 <- aux;
+      leakages <- LeakAddr([]) :: leakages;
+      aux <- x1;
+      leakages <- LeakAddr([i]) :: leakages;
+      a.[i] <- aux;
+      i <- i + 1;
+    }
+    return (cf, a);
+  }
+  
+  proc rsample (byte_z:W64.t Array32.t) : int * W64.t Array32.t = {
+    var aux_1: bool;
+    var aux_0: int;
+    var aux: W64.t;
+    var aux_2: W8.t Array256.t;
+    var aux_3: W64.t Array32.t;
+    
+    var i:int;
+    var byte_p:W64.t Array32.t;
+    var q0:W64.t;
+    var q1:W64.t;
+    var z:bool;
+    var byte_q:W64.t Array32.t;
+    var cf:bool;
+    byte_p <- witness;
+    byte_q <- witness;
+    leakages <- LeakAddr([]) :: leakages;
+    aux <- (W64.of_int 0);
+    q0 <- aux;
+    leakages <- LeakAddr([]) :: leakages;
+    aux <- (W64.of_int 1);
+    q1 <- aux;
+    leakages <- LeakAddr([]) :: leakages;
+    aux_0 <- 0;
+    i <- aux_0;
+    leakages <- LeakAddr([]) :: leakages;
+    aux_1 <- (q0 = (W64.of_int 0));
+    z <- aux_1;
+    
+    leakages <- LeakCond(z) :: LeakAddr([]) :: leakages;
+    
+    while (z) {
+      leakages <- LeakAddr([]) :: leakages;
+      aux_2 <@ SC.randombytes_256 ((Array256.init (fun i_0 => get8
+                                   (WArray256.init64 (fun i_0 => byte_p.[i_0]))
+                                   i_0)));
+      byte_p <-
+      (Array32.init (fun i_0 => get64
+      (WArray256.init8 (fun i_0 => aux_2.[i_0])) i_0));
+      leakages <- LeakAddr([]) :: leakages;
+      (aux_1, aux_3) <@ bn_subc (byte_q, byte_z);
+      cf <- aux_1;
+      byte_q <- aux_3;
+      leakages <- LeakAddr([]) :: leakages;
+      aux <- (cf ? q1 : q0);
+      q0 <- aux;
+      leakages <- LeakAddr([]) :: leakages;
+      aux_1 <- (q0 = (W64.of_int 1));
+      z <- aux_1;
+      leakages <- LeakAddr([]) :: leakages;
+      aux_0 <- (i + 1);
+      i <- aux_0;
+    leakages <- LeakCond(z) :: LeakAddr([]) :: leakages;
+    
+    }
+    return (i, byte_p);
+  }
+  
+  proc toEC () : unit = {
+    var aux: int;
+    var aux_0: W64.t Array32.t;
+    
+    var a:W64.t Array32.t;
+    var r:W64.t Array32.t;
+    var  _0:int;
+    a <- witness;
+    r <- witness;
+    leakages <- LeakAddr([]) :: leakages;
+    (aux, aux_0) <@ rsample (a);
+     _0 <- aux;
+    r <- aux_0;
+    return ();
+  }
+}.
+
