proof/Uniform_distr_proof_ct.ec
@@ -1,0 +1,84 @@
+require import Ring_ops_extract_ct.
+require import JModel List Int AllCore.
+
+
+require import Array1.
+require import WArray1.
+
+require import Uniform_distr_extract_ct.
+
+op sub_prefix : leakages_t = 
+  [LeakFor (1, 32); LeakAddr []; LeakAddr [0]; LeakAddr []; 
+    LeakAddr []; LeakAddr [0]; LeakAddr [0]].
+
+op sub_step (i : int) : leakages_t = 
+  [LeakAddr [i] ; LeakAddr [] ; LeakAddr [] ; LeakAddr [i] ; 
+    LeakAddr [i] ].
+
+
+op sub_g (x : int) : leakages_t.
+axiom sub_g_comp_1 x : 1 <= x  => sub_g x = [].
+axiom sub_g_comp_2 x : 1 < x => sub_g x = sub_step (x-1) ++ sub_g (x - 1).
+
+op sub_f (x : int) : leakages_t = sub_g x ++ sub_prefix.
+
+
+
+lemma jj start_l :
+   hoare [ M(Syscall).bn_subc : M.leakages = start_l ==> M.leakages = sub_f 32 ++ start_l ].
+proof. 
+proc.
+sp.  elim*. progress.
+conseq (_: M.leakages = sub_prefix ++ start_l /\ i = 1 ==> _).
+progress.
+while (0 < i /\ i <= 32 /\ M.leakages = sub_f i ++ start_l).
+wp.  skip.  progress. 
+simplify. smt(). smt(). rewrite /sub_f. rewrite (sub_g_comp_2 (i{hr} +1)).  smt(). simplify. rewrite /sub_step. simplify. auto.
+skip. progress. rewrite /sub_f.  rewrite sub_g_comp_1. auto. auto.
+smt().
+qed.
+
+
+op samp_prefix : leakages_t = 
+  LeakCond true :: LeakAddr [] :: LeakAddr [] :: LeakAddr [] :: LeakAddr [] :: 
+  LeakAddr [] :: [].
+op samp_g (x : int) : leakages_t.
+op samp_step (i : int) : leakages_t = LeakCond true :: LeakAddr [] :: LeakAddr [] :: LeakAddr [] :: LeakAddr [] :: (
+sub_f 32 ++ LeakAddr [] :: LeakAddr [] :: []).
+
+  
+
+axiom samp_g_comp_1 x : 0 <= x  => samp_g x = [].
+axiom samp_g_comp_2 x : 0 < x => samp_g x = samp_step (x-1) ++ samp_g (x - 1).
+
+op samp_suffix : leakages_t = 
+ LeakCond false :: LeakAddr [] :: LeakAddr [] :: LeakAddr [] :: LeakAddr [] :: 
+sub_f 32 ++ LeakAddr [] :: LeakAddr [] :: [].
+
+op samp_f (x : int) : leakages_t = samp_g x ++ samp_prefix.
+op samp_t (x : int) : leakages_t = samp_suffix ++ samp_f (x - 1).
+
+
+
+lemma ii :
+   hoare [ M(Syscall).rsample : M.leakages = [] ==> M.leakages = samp_t res.`1].
+proc.
+sp. elim*. progress.
+conseq (_: M.leakages = samp_prefix /\ i = 0  /\ z = true ==> _).
+progress.
+while (0 <= i /\ (z = true => M.leakages = samp_f i) 
+              /\ (z = false => M.leakages = samp_t i)).
+wp. 
+ecall (jj M.leakages). wp. inline*. wp. rnd. wp.  skip. progress.
+smt().  rewrite H4.  rewrite H0. rewrite H2. auto.
+rewrite /samp_f. rewrite (samp_g_comp_2 (i{hr} + 1)). smt().
+simplify. rewrite /samp_step.   
+smt(@List). rewrite H4. rewrite H0. rewrite H2. auto.
+rewrite /samp_t. simplify.
+rewrite /samp_suffix. smt(@List).
+skip. progress. rewrite /samp_prefix. rewrite /samp_f. rewrite samp_g_comp_1.
+auto. rewrite /samp_prefix. auto.
+rewrite H2. rewrite H. auto.
+auto.
+qed.
+    
