proof/eclib/Array1.ec
@@ -1,0 +1,3 @@
+require import JArray.
+
+clone export PolyArray as Array1  with op size <- 1.
