proof/eclib/Array256.ec
@@ -1,0 +1,3 @@
+require import JArray.
+
+clone export PolyArray as Array256  with op size <- 256.
