proof/eclib/WArray1.ec
@@ -1,0 +1,3 @@
+require import JWord_array.
+
+clone export WArray as WArray1  with op size <- 1.
